cleanup

Imp/Untyped/Aexp.lean
@@ -6,43 +6,44 @@ import Mathlib.Init.Function
 namespace Aexp
 
 -- Operational semantics of aexp
-inductive Nat: Aexp × State → Val → Prop
+inductive Natural: Aexp × State → Val → Prop
   | num₁:
-    Nat (num n, _) n
+    Natural (num n, _) n
 
   | loc₁:
-    Nat (loc x, s) (s x)
+    Natural (loc x, s) (s x)
 
-  | add₁ (h₁: Nat (a,s) n) (h₂: Nat (b,s) m):
-    Nat (add a b, s) (n + m)
+  | add₁ (h₁: Natural (a,s) n) (h₂: Natural (b,s) m):
+    Natural (add a b, s) (n + m)
 
-  | sub₁ (h₁: Nat (a,s) n) (h₂: Nat (b,s) m):
-    Nat (sub a b, s) (n - m)
+  | sub₁ (h₁: Natural (a,s) n) (h₂: Natural (b,s) m):
+    Natural (sub a b, s) (n - m)
 
-  | mul₁ (h₁: Nat (a,s) n) (h₂: Nat (b,s) m):
-    Nat (mul a b, s) (n * m)
+  | mul₁ (h₁: Natural (a,s) n) (h₂: Natural (b,s) m):
+    Natural (mul a b, s) (n * m)
 
-infix:110 " ⟹ " => Nat
+infix:110 " ⟹ " => Natural
 
 -- Denotational semantics of arithmetic expressions
-@[reducible] def red (a: Aexp) (s: State): Val :=
+@[reducible]
+def reduce (a: Aexp) (s: State): Val :=
   match a with
   | num n => n
   | loc x => s x
-  | add a b => red a s + red b s
-  | sub a b => red a s - red b s
-  | mul a b => red a s * red b s
+  | add a b => reduce a s + reduce b s
+  | sub a b => reduce a s - reduce b s
+  | mul a b => reduce a s * reduce b s
 
-infix:110 "⇓" => red
+infix:110 "⇓" => reduce
 
 -- relational definition is equal to recursive
-theorem red.from_Nat (h: as ⟹ n): red.uncurry as = n :=
+theorem reduce.from_Natural (h: as ⟹ n): reduce.uncurry as = n :=
   by induction h with
   | num₁ => rfl
   | loc₁ => rfl
   | _ _ _ ih₁ ih₂ => exact ih₁ ▸ ih₂ ▸ rfl
 
-theorem Nat.from_red {a: Aexp} (h: a⇓s = n): (a,s) ⟹ n :=
+theorem Natural.from_reduce {a: Aexp} (h: a⇓s = n): (a,s) ⟹ n :=
   by induction a generalizing n with
   | num _ => exact h ▸ num₁
   | loc _ => exact h ▸ loc₁
@@ -50,10 +51,10 @@ theorem Nat.from_red {a: Aexp} (h: a⇓s = n): (a,s) ⟹ n :=
   | sub _ _ l r => exact h ▸ sub₁ (l rfl) (r rfl)
   | mul _ _ l r => exact h ▸ mul₁ (l rfl) (r rfl)
 
-@[simp] theorem Nat_iff_red: (a, s) ⟹ n ↔ a⇓s = n := ⟨red.from_Nat, Nat.from_red⟩
-@[simp] theorem Nat_iff_red': (a, s) ⟹ (a⇓s) := Nat.from_red rfl
+@[simp] theorem Natural_iff_reduce: (a, s) ⟹ n ↔ a⇓s = n := ⟨reduce.from_Natural, Natural.from_reduce⟩
+@[simp] theorem Natural_iff_reduce': (a, s) ⟹ (a⇓s) := Natural.from_reduce rfl
 
-protected instance Nat.equiv: Setoid Aexp where
+protected instance Natural.equiv: Setoid Aexp where
   r a b := ∀ s n, (a, s) ⟹ n = (b, s) ⟹ n
   iseqv := {
     refl := λ _ _ _ ↦ Eq.refl _
@@ -61,11 +62,11 @@ protected instance Nat.equiv: Setoid Aexp where
     trans := λ h₁ h₂ x n ↦ (h₁ x n) ▸ (h₂ x n)
   }
 
-instance red.equiv: Setoid Aexp where
+instance reduce.equiv: Setoid Aexp where
   r a b := ∀s, a⇓s = b⇓s
   iseqv := ⟨λ _ _ ↦ Eq.refl _, (Eq.symm $ · ·) , λ h₁ h₂ s ↦ (h₁ s) ▸ (h₂ s)⟩
 
-protected theorem Nat_eq_eq_red_eq: Nat.equiv.r a b ↔ red.equiv.r a b := by
+protected theorem Natural_eq_eq_reduce_eq: Natural.equiv.r a b ↔ reduce.equiv.r a b := by
   constructor <;> intro h
   . simp [Setoid.r] at *
     intro s
